proved that fwded proposals are in propCmd.

Isabelle2/R3_Refines_R1.thy
@@ -82,26 +82,24 @@ lemmas ioa_defs =
    IOA.actions_def
    IOA.externals_def IOA.add_history_def
 
+definition update where "update s h a s' \<equiv> case a of 
+  Propose v \<Rightarrow> h\<lparr>propCmd := insert v (propCmd h)\<rparr>
+  | Internal \<Rightarrow> 
+      h\<lparr>vote := \<lambda> i a b . case (votes (lstate s' a) $ i) of Some (v,b2) \<Rightarrow> 
+          (if b = b2 then Some v else (vote h i a b)) | None \<Rightarrow> None,
+        ampr1_state.ballot := \<lambda> a . local_state.ballot (lstate s' a),
+        suggestion := \<lambda> i b . case (log (lstate s' (leader b)) $ i) of Proposed v \<Rightarrow> (
+              case (log (lstate s (leader b)) $ i) of Free \<Rightarrow> Some v | _ \<Rightarrow> suggestion h i b)
+          | Decided v \<Rightarrow> suggestion h i b
+          | Free \<Rightarrow> None,
+        onebs := \<lambda> a b . if local_state.ballot (lstate s' a) = b \<and> local_state.ballot (lstate s' a) \<noteq> b
+          then Some (op$ (votes (lstate s a))) else None\<rparr>
+  | _ \<Rightarrow> h"
+
 definition ghost_ioa where 
   -- {* This gets a little tricky. Why not define a history IOA without @{term add_hist} and 
   prove trace inclusion with a forward simulation? *}
-  "ghost_ioa \<equiv>
-      let update = \<lambda> s h a s' . case a of 
-        Propose v \<Rightarrow> h\<lparr>propCmd := insert v (propCmd h)\<rparr>
-        | Internal \<Rightarrow> 
-            h\<lparr>vote := \<lambda> i a b . case (votes (lstate s' a) $ i) of Some (v,b2) \<Rightarrow> 
-                (if b = b2 then Some v else (vote h i a b)) | None \<Rightarrow> None,
-              ampr1_state.ballot := \<lambda> a . local_state.ballot (lstate s' a),
-              suggestion := \<lambda> i b . case (log (lstate s' (leader b)) $ i) of Proposed v \<Rightarrow> (
-                    case (log (lstate s (leader b)) $ i) of Free \<Rightarrow> Some v | _ \<Rightarrow> suggestion h i b)
-                | Decided v \<Rightarrow> suggestion h i b
-                | Free \<Rightarrow> None,
-              onebs := \<lambda> a b . if local_state.ballot (lstate s' a) = b \<and> local_state.ballot (lstate s' a) \<noteq> b
-                then Some (op$ (votes (lstate s a))) else None\<rparr>
-        | _ \<Rightarrow> h;
-        init = \<lambda> s . r1.start_s
-      in
-    add_history ampr3_ioa update init"
+  "ghost_ioa \<equiv> add_history ampr3_ioa update (\<lambda> s . r1.start_s)"
 
 lemmas amp_defs = ioa_defs ampr1_ioa_def ampr3_ioa_def ghost_ioa_def
   ioa_def global_start_def
@@ -110,7 +108,7 @@ definition inv1 where "inv1 s \<equiv> let r3_s = fst s; h = snd s in
   \<forall> a v . (Packet a (Fwd v)) \<in> network r3_s \<longrightarrow> v \<in> propCmd h"
 declare inv1_def[inv_proofs_defs]
 
-lemma inv2:"invariant ghost_ioa inv1"
+lemma inv1:"invariant ghost_ioa inv1"
   apply (rule invariantI)
    apply (simp add:inv1_def amp_defs)
   apply (rm_reachable)
@@ -118,7 +116,25 @@ lemma inv2:"invariant ghost_ioa inv1"
   apply (simp only: split_paired_all)
   apply (frule IOA.add_hist_trans(1), drule IOA.add_hist_trans(2))
   apply (simp add:is_trans_def ampr3_ioa_def ioa_def)
-  apply (drule trans_cases) oops
+  apply (elim trans_cases)
+         apply (auto simp add:inv1_def update_def)
+         apply (simp add:propose_def do_2a_def Let_def send_all_def split:if_splits)
+        apply (simp add:receive_2b_def Let_def send_all_def split:if_splits)
+       apply (simp add:try_acquire_leadership_def Let_def send_all_def split:if_splits)
+      apply (simp add:receive_1a_def Let_def send_all_def split:if_splits)
+     apply (simp add:receive_2a_def Let_def send_all_def split:if_splits)
+    apply (simp add:receive_2b_def Let_def send_all_def split:if_splits)
+   apply (simp add:receive_1b_def Let_def send_all_def msgs_def receive_1b.msgs_def split:if_splits)
+  subgoal proof -
+    fix a :: "('a, 'v) global_state" and b :: "('v, 'a, ?'l) ampr1_state" and ac :: 'a and bb :: nat and vs :: "nat \<Rightarrow>f ('v \<times> nat) option" and ad :: "('a, 'v) local_state" and bc :: "('a, 'v) packet set" and ae :: 'a and v :: 'v
+    assume a1: "(\<exists>x. finfun_dom (receive_1b.new_log (the (local_state.onebs (lstate a ac) $ bb)) (acceptors (lstate a ac)) (log (lstate a ac))) $ x \<and> (Fwd v::('a, 'v) msg) = (case the_elem (receive_1b.max_per_inst (the (local_state.onebs (lstate a ac) $ bb)) (acceptors (lstate a ac)) $ x) of (v, b) \<Rightarrow> Phase2a x b v)) \<and> ae \<in> acceptors (lstate a ac) \<and> ae \<noteq> local_state.id (lstate a ac)"
+    have "\<And>n p v. (case p of (v, na) \<Rightarrow> Phase2a n na v) \<noteq> (Fwd v::('a, 'v) msg)"
+      by (metis amp_r3.msg.distinct(17) case_prod_conv surj_pair)
+    then show "v \<in> propCmd b"
+      using a1 by metis
+  qed
+  apply (simp add:receive_fwd_def do_2a_def Let_def send_all_def split:if_splits)
+  done
   
 definition ref_map where "ref_map s \<equiv> snd s"
   
